src/Analyze/AbstractInterpCpsK.v
@@ -11,19 +11,21 @@ Require Import CoqCompile.TraceMonad.
 
 Import CpsK.CPSK.
 
+Set Implicit Arguments.
+Set Strict Implicit.
+
 Section AI.
   Variables D C V : Type.
   Context {AbsTime_C  : AbsTime C}.
-  Context {AbsValue_V : AbsDomain D V C (var + cont)}.
+  Context {AbsValue_V : AbsDomain C D (var + cont) V}.
   Context {IntValue_V : IntValue V}.
   Context {BoolValue_V : BoolValue V}.
   Context {CtorValue_V  : CtorValue V constructor}.
-  Context {FnValue_V  : FnValue (var + cont) V C D}.
-  Context {TplValue_V : TplValue V (list V)}.
+  Context {FnValue_V  : FnValue C D (var + cont) V}.
+  Context {TplValue_V : TplValue C D V}.
   Context {Show_C : Show C}.
   Context {Show_D : Show D}.
   Context {Show_V : Show V}.
-  Context {RelDec_V : RelDec (@eq V)}.
 
   Import MonadNotation.
   Local Open Scope monad_scope.
@@ -36,7 +38,6 @@ Section AI.
     Context {Fix_m : MonadFix m}.
     (** DFS **)
     Context {State_m : MonadState (alist (C * exp) D) m}.
-    Context {Aheap_m : MonadState (alist V (list V)) m}.
     Context {Trace_m : MonadTrace string m}.
 
     Definition eval_op (o : op) (ctx : C) (dom : D) : m V :=
@@ -51,65 +52,47 @@ Section AI.
     Definition illFormed_decl {A} (d : decl) : m A :=
       raise ("Ill-formed declaration " ++ runShow (show d))%string.
 
-    Locate alist.
-
     Definition eval_decl (d : decl) (ctx : C) (dom : D) : m D :=
-      v_vA <- 
-      match d return m (list (var * V)) with
-        | Op_d v o =>
-          oA <- eval_op o ctx dom ;;
-          ret ((v, oA) :: nil)
-            
-        | Prim_d v p os => 
-          argsA <- mapM (fun x => eval_op x ctx dom) os ;;
-          vA <- match p , argsA with
-                  | Eq_p , l :: r :: nil =>
-                    ret (injBool (eqA l r))
-                  | Neq_p , l :: r :: nil =>
-                    ret (injBool (map negb (eqA l r)))
-                  | Lt_p , l :: r :: nil =>
-                    ret (injBool (ltA l r))
-                  | Lte_p , l :: r :: nil =>
-                    ret (orA (injBool (ltA l r)) (injBool (eqA l r)))
-                  | Ptr_p , l :: nil => ret (injBool None) (** ?? **)
-                  | Plus_p , l :: r :: nil => ret (plusA l r)
-                  | Minus_p , l :: r :: nil => ret (minusA l r)
-                  | Times_p , l :: r :: nil => ret (timesA l r)
-                  | MkTuple_p , argsA => 
-                    aheap <- get ;;
-                    let aloc := injTuple aheap v argsA in
-                    match Maps.lookup aloc aheap with
-                      | None => modify (Maps.add aloc argsA)
-                      | Some v => modify (Maps.add aloc argsA) (* TODO: need to pointwise join *)
-                    end ;;
-                    ret aloc
-                    (* ret (injTuple aheap v argsA) *)
-                  | Proj_p , l :: r :: nil => 
-                    aheap <- get ;;
-                    ret (projA aheap l r)
-                  | _ , _ => illFormed_decl (Prim_d v p os)
-                end ;;
-          ret ((v, vA) :: nil)
-
-        | Fn_d v ks args body =>
-          ret ((v, injFn ctx (inl v) ks args body) :: nil)
-          
-        | Bind_d v1 v2 m os =>
-          ret ((v1, topA) :: (v2, topA) :: nil)
-      end ;;
-      let dom' := fold_left (fun dom v_vA => let '(v, vA) := v_vA in
-        update ctx (inl v) vA dom) v_vA dom in
-      ret dom'.
-
-    Definition init_decl (d : decl) (ctx : C) (dom : D) : D :=
       match d with
-        | Op_d v _ 
-        | Prim_d v _ _
-        | Fn_d v _ _ _ => 
-          update ctx (inl v) bottomA dom
-        | Bind_d v1 v2 _ _ =>
-          let dom := update ctx (inl v1) bottomA dom in
-            update ctx (inl v2) bottomA dom
+        | Prim_d v Mk_tuple os =>
+          argsA <- mapM (fun x => eval_op x ctx dom) os ;;
+          ret (injTuple dom ctx v argsA)
+        | _ =>
+          v_vA <- 
+          match d return m (list (var * V)) with
+            | Op_d v o =>
+              oA <- eval_op o ctx dom ;;
+              ret ((v, oA) :: nil)
+              
+            | Prim_d v p os => 
+              argsA <- mapM (fun x => eval_op x ctx dom) os ;;
+              vA <- match p , argsA with
+                      | Eq_p , l :: r :: nil =>
+                        ret (injBool (eqA l r))
+                      | Neq_p , l :: r :: nil =>
+                        ret (injBool (map negb (eqA l r)))
+                      | Lt_p , l :: r :: nil =>
+                        ret (injBool (ltA l r))
+                      | Lte_p , l :: r :: nil =>
+                        ret (orA (injBool (ltA l r)) (injBool (eqA l r)))
+                      | Ptr_p , l :: nil => ret (injBool None) (** ?? **)
+                      | Plus_p , l :: r :: nil => ret (plusA l r)
+                      | Minus_p , l :: r :: nil => ret (minusA l r)
+                      | Times_p , l :: r :: nil => ret (timesA l r)
+                      | Proj_p , l :: r :: nil => ret (projA dom l r)
+                      | _ , _ => illFormed_decl (Prim_d v p os)
+                    end ;;
+              ret ((v, vA) :: nil)
+              
+            | Fn_d v ks args body =>
+              ret ((v, injFn ctx (inl v) ks args body) :: nil)
+              
+            | Bind_d v1 v2 m os =>
+              ret ((v1, topA) :: (v2, topA) :: nil)
+          end ;;
+          let dom' := fold_left (fun dom v_vA => let '(v, vA) := v_vA in
+            update ctx (inl v) vA dom) v_vA dom in
+          ret dom'
       end.
 
     Local Open Scope string_scope.
@@ -142,7 +125,7 @@ Section AI.
           modify (Maps.add (ctx, e) dom) ;;
           MAP <- get ;;
           let len : nat := length MAP in
-          mlog ("adding shit to map " ++ to_string (len)) ;;
+          mlog ("adding stuff to map " ++ to_string (len)) ;;
           (fix recur (ctx : C) (dom : D) (e : exp) : m D :=
             match e return m D with
               | App_e o ks os =>
@@ -165,9 +148,10 @@ Section AI.
                     update ctx (inr k) (injFn ctx (inr k) nil xs e) dom) ks dom in
                 recur ctx dom' e
               | Letrec_e ds e =>
-                let dom_init := 
-                  fold_left (fun dom d => init_decl d ctx dom) ds dom in
-                dom' <- foldM (fun d dom => eval_decl d ctx dom) (ret dom_init) ds ;;
+                dom' <- 
+                mfix (fun go => fun (dom : D) =>
+                  dom' <- foldM (fun d acc => eval_decl d ctx acc) (ret dom) ds ;;
+                  if dom_leq dom' dom then ret dom' else go dom') dom ;;
                 recur ctx dom' e
               | Switch_e o arms e =>
                 s <- eval_op o ctx dom ;;
@@ -183,8 +167,6 @@ Section AI.
                 mlog "got to halt"%string ;;
                 ret dom
             end) ctx dom e).
-
-    Print aeval_exp.
     
   End Monadic.
 
@@ -193,7 +175,7 @@ Section AI.
   Require Import ExtLib.Data.Monads.FuelMonad.
   Require Import ExtLib.Data.Monads.IdentityMonad.
 
-  Arguments aeval_exp {m} {_ _ _ _ _ _} ctx dom e.
+  Arguments aeval_exp {m} {_ _ _ _ _} ctx dom e.
   
   Section interface.
     Variable m : Type -> Type.
@@ -202,8 +184,8 @@ Section AI.
 
     Require Import BinNums.
     Definition aeval (ctx : C) (dom : D) (e : exp) (fuel : N) : m (string + D) :=
-      let c := aeval_exp (m := GFixT (eitherT string (stateT (alist (C * exp) D) (stateT (alist V (list V)) m)))) ctx dom e in 
-      bind (evalStateT (evalStateT (unEitherT (runGFixT c fuel)) Maps.empty) Maps.empty) (fun res => 
+      let c := aeval_exp (m := GFixT (eitherT string (stateT (alist (C * exp) D) m))) ctx dom e in 
+      bind (evalStateT (unEitherT (runGFixT c fuel)) Maps.empty) (fun res => 
       match res with
         | inl err => ret (inl err)
         | inr None => ret (inl "aeval: out of fuel")%string
@@ -212,3 +194,4 @@ Section AI.
   End interface.
 
 End AI.
+
